disable optimization of disjointness indexes; treated the same way as eloc and inv; things work again

src/3d/InterpreterTarget.fst
@@ -43,6 +43,7 @@ type disj_pre =
   | Disj_triv : disj_pre
   | Disj_pair : eloc -> eloc -> disj_pre
   | Disj_conj : disj_pre -> disj_pre -> disj_pre
+  | Disj_name : A.ident -> list expr -> disj_pre
 
 let rec subst_eloc subst (e:eloc)
   : eloc
@@ -67,12 +68,14 @@ let rec subst_disj_index subst (d:disj_pre)
     | Disj_conj d1 d2 ->
       Disj_conj (subst_disj_index subst d1)
                 (subst_disj_index subst d2)
+    | Disj_name hd args ->
+      Disj_name hd (List.Tot.map (T.subst_expr subst) args)
 
-let disj_conj d0 d1 =
-  match d0, d1 with
-  | Disj_triv, d
-  | d, Disj_triv -> d
-  | _, _ -> Disj_conj d0 d1
+let disj_conj d0 d1 = Disj_conj d0 d1
+  // match d0, d1 with
+  // | Disj_triv, d
+  // | d, Disj_triv -> d
+  // | _, _ -> Disj_conj d0 d1
 
 noeq
 type on_success =
@@ -84,9 +87,19 @@ let typ_indexes = inv & eloc & disj_pre & on_success
 let typ_indexes_nil = Inv_true, Eloc_none, Disj_triv, On_success false
 let typ_indexes_union (i, e, d, b) (i', e', d', b') =
   Inv_conj i i', Eloc_union e e', disj_conj d d', On_success_union b b'
-let typ_indexes_name_except_disj hd args =
+let typ_indexes_union_l_bias (i, e, d, b) (i', e', d', b') =
+  if not (Disj_triv? d)
+  then failwith "Unexpected disjunctive index in typ_indexes_union_l_bias"
+  else Inv_conj i i', Eloc_union e e', d', On_success_union b b'
+let typ_indexes_union_r_bias (i, e, d, b) (i', e', d', b') =
+  if not (Disj_triv? d')
+  then failwith "Unexpected disjunctive index in typ_indexes_union_r_bias"
+  else Inv_conj i i', Eloc_union e e', d, On_success_union b b'
+ 
+let typ_indexes_name hd args =
   Inv_name hd args,
   Eloc_name hd args,
+  Disj_name hd args,
   On_success_named hd args
 
 let env = H.t A.ident' type_decl
@@ -271,23 +284,24 @@ let rec typ_indexes_of_parser (en:env) (p:T.parser)
           | Some td -> td
           | _ -> failwith (Printf.sprintf "Type decl not found for %s" (A.ident_to_string hd))
         in
-        let _, _, disj_index_p, _ = td.typ_indexes in
-        let subst =
-          match T.mk_subst td.name.td_params args with
-          | None -> 
-            failwith (Printf.sprintf "Unexpected number of arguments to type %s" (A.ident_to_string td.name.td_name))
-          | Some s -> s
-        in
-        let disj_index = subst_disj_index subst disj_index_p in
-        let i, e, r = typ_indexes_name_except_disj hd (filter_args_for_inv args td) in
-        i, e, disj_index, r
+        // let _, _, disj_index_p, _ = td.typ_indexes in
+        // let subst =
+        //   match T.mk_subst td.name.td_params args with
+        //   | None -> 
+        //     failwith (Printf.sprintf "Unexpected number of arguments to type %s" (A.ident_to_string td.name.td_name))
+        //   | Some s -> s
+        // in
+        // let disj_index = subst_disj_index subst disj_index_p in
+        typ_indexes_name hd (filter_args_for_inv args td)
       end
 
     | T.Parse_if_else _ p q
-    | T.Parse_pair _ p q
+    | T.Parse_pair _ p q ->
+      typ_indexes_union (typ_indexes_of_parser p) (typ_indexes_of_parser q)
+
     | T.Parse_dep_pair _ p (_, q)
     | T.Parse_dep_pair_with_refinement _ p _ (_, q) ->
-      typ_indexes_union (typ_indexes_of_parser p) (typ_indexes_of_parser q)
+      typ_indexes_union_l_bias (typ_indexes_of_parser p) (typ_indexes_of_parser q)
 
     | T.Parse_weaken_left p _
     | T.Parse_weaken_right p _
@@ -300,18 +314,20 @@ let rec typ_indexes_of_parser (en:env) (p:T.parser)
 
     | T.Parse_dep_pair_with_action p (_, a) (_, q)
     | T.Parse_dep_pair_with_refinement_and_action _ p _ (_, a) (_, q) ->
-      typ_indexes_union (typ_indexes_of_parser p)
-                     (typ_indexes_union (typ_indexes_of_action a) (typ_indexes_of_parser q))
+      typ_indexes_union_l_bias (typ_indexes_of_parser p)
+                     (typ_indexes_union_l_bias (typ_indexes_of_action a) (typ_indexes_of_parser q))
 
-    | T.Parse_with_action _ p a
+    | T.Parse_with_action _ p a ->
+      typ_indexes_union_r_bias (typ_indexes_of_parser p) (typ_indexes_of_action a)
+
     | T.Parse_with_dep_action _ p (_, a) ->
-      typ_indexes_union (typ_indexes_of_parser p) (typ_indexes_of_action a)
+      typ_indexes_union_l_bias (typ_indexes_of_parser p) (typ_indexes_of_action a)
 
     | T.Parse_string p _ ->
       typ_indexes_nil
 
     | T.Parse_refinement_with_action n p f (_, a) ->
-      typ_indexes_union (typ_indexes_of_parser p) (typ_indexes_of_action a)
+      typ_indexes_union_l_bias (typ_indexes_of_parser p) (typ_indexes_of_action a)
 
     | T.Parse_with_probe p _ _ dest ->
       let i, l, d, s = typ_indexes_of_parser p in 
@@ -773,12 +789,12 @@ let rec print_eloc mname (e:eloc)
 let rec print_disj mname (d:disj_pre)
   : ML string
   = match d with
-    | Disj_triv -> "None"
-    | Disj_pair i j -> Printf.sprintf "(Some (A.disjoint %s %s))" (print_eloc mname i) (print_eloc mname j)
+    | Disj_triv -> "disj_none"
+    | Disj_pair i j -> Printf.sprintf "(A.disjoint %s %s)" (print_eloc mname i) (print_eloc mname j)
     | Disj_conj i j -> Printf.sprintf "(join_disj %s %s)" (print_disj mname i) (print_disj mname j)
-    // | Disj_name hd args -> Printf.sprintf "(%s %s)" (print_derived_name mname "disj" hd) (print_args mname args)
+    | Disj_name hd args -> Printf.sprintf "(%s %s)" (print_derived_name mname "disj" hd) (print_args mname args)
 
-let print_td_iface is_entrypoint mname root_name binders args typ_indexes_binders typ_indexes_args disj_index ar pk_wk pk_nz =
+let print_td_iface is_entrypoint mname root_name binders args typ_indexes_binders typ_indexes_args ar pk_wk pk_nz =
   let kind_t =
     Printf.sprintf "[@@noextract_to \"krml\"]\n\
                     inline_for_extraction\n\
@@ -795,6 +811,13 @@ let print_td_iface is_entrypoint mname root_name binders args typ_indexes_binder
       root_name
       typ_indexes_binders
   in
+  let disj_t =
+    Printf.sprintf "[@@noextract_to \"krml\"]\n\
+                    noextract\n\
+                    val disj_%s %s : disj_index"
+      root_name
+      typ_indexes_binders
+  in
   let eloc_t =
     Printf.sprintf "[@@noextract_to \"krml\"]\n\
                     noextract\n\
@@ -805,12 +828,12 @@ let print_td_iface is_entrypoint mname root_name binders args typ_indexes_binder
   let def'_t =
     Printf.sprintf "[@@noextract_to \"krml\"]\n\
                     noextract\n\
-                    val def'_%s %s: typ kind_%s (inv_%s %s) (%s) (eloc_%s %s) %b"
+                    val def'_%s %s: typ kind_%s (inv_%s %s) (disj_%s %s) (eloc_%s %s) %b"
       root_name
       binders
       root_name
       root_name typ_indexes_args
-      disj_index //root_name typ_indexes_args
+      root_name typ_indexes_args
       root_name typ_indexes_args
       ar
   in
@@ -829,7 +852,7 @@ let print_td_iface is_entrypoint mname root_name binders args typ_indexes_binder
       binders
       root_name args
   in
-  String.concat "\n\n" [kind_t; inv_t; eloc_t; def'_t; validator_t; dtyp_t]
+  String.concat "\n\n" [kind_t; inv_t; disj_t; eloc_t; def'_t; validator_t; dtyp_t]
 
 let print_binders mname binders =
     List.map (print_param mname) binders |>
@@ -906,14 +929,15 @@ let print_binding mname (td:type_decl)
       (T.print_kind mname k)]
   in
   let print_inv_or_eloc_or_disj = print_inv_or_eloc_or_disj mname tdn root_name binders in
-  let typ_indexes_of_binding, disj_index, fv_binders, fv_args =
+  let typ_indexes_of_binding, fv_binders, fv_args =
     let inv, eloc, disj, _ = td.typ_indexes in
     let fvs1 = free_vars_of_inv inv in
     let fvs2 = free_vars_of_disj disj in
     let fvs3 = free_vars_of_eloc eloc in
     let s0, _, _ = print_inv_or_eloc_or_disj "inv" None "A.slice_inv" (print_inv mname inv) (fvs1@fvs2@fvs3) in
+    let s1, _, _ = print_inv_or_eloc_or_disj "disj" None "disj_index" (print_disj mname disj) (fvs1@fvs2@fvs3) in
     let s2, fvb, fva = print_inv_or_eloc_or_disj "eloc" None "A.eloc" (print_eloc mname eloc) (fvs1@fvs2@fvs3) in
-    s0 ^ s2, print_disj mname disj, fvb, fva
+    s0 ^ s1 ^ s2, fvb, fva
   in
   let def' =
     OS.format
@@ -1035,7 +1059,7 @@ let print_binding mname (td:type_decl)
     let iface =
       print_td_iface td.name.td_entrypoint
                     mname root_name binders args
-                    fv_binders fv_args disj_index td.allow_reading
+                    fv_binders fv_args td.allow_reading
                     weak_kind k.pk_nz
     in
     impl, iface
